src/simulation/Knot2Glob.v
@@ -599,7 +599,7 @@ Section PROOF.
       eapply IH; eauto.
     }
 
-    { destruct KSIM0 as [KSIM0 IND]. rewrite interp_all_rmw.
+    { destruct KSIM0 as [KSIM0 IND]. rewrite interp_all_state.
       do 2 (guclo sim_indC_spec; eapply sim_indC_tauL).
       eapply IH; eauto.
     }
@@ -631,7 +631,7 @@ Section PROOF.
       eapply IH; eauto.
     }
 
-    { destruct KSIM0 as [KSIM0 IND]. rewrite interp_all_rmw.
+    { destruct KSIM0 as [KSIM0 IND]. rewrite interp_all_state.
       do 2 (guclo sim_indC_spec; eapply sim_indC_tauR).
       eapply IH; eauto.
     }
@@ -763,7 +763,7 @@ Section PROOF.
       eapply IH; eauto.
     }
 
-    { destruct KSIM0 as [KSIM0 IND]. rewrite interp_all_rmw.
+    { destruct KSIM0 as [KSIM0 IND]. rewrite interp_all_state.
       do 2 (guclo sim_indC_spec; eapply sim_indC_tauL).
       eapply IH; eauto.
     }
@@ -795,7 +795,7 @@ Section PROOF.
       eapply IH; eauto.
     }
 
-    { destruct KSIM0 as [KSIM0 IND]. rewrite interp_all_rmw.
+    { destruct KSIM0 as [KSIM0 IND]. rewrite interp_all_state.
       do 2 (guclo sim_indC_spec; eapply sim_indC_tauR).
       eapply IH; eauto.
     }
